Coupon more stuff

theories/examples/coupon.v
@@ -4,38 +4,103 @@ From clutch.lib Require Export map.
 
 Set Default Proof Using "Type*".
 
+
+Definition cnt_map_helper : expr :=
+    (rec: "cnt_helper" "m" "k" "n" :=
+       if: "k" = "n"
+       then #0
+       else
+         match: get "m" "k" with
+           NONE => "cnt_helper" "m" ("k"+#1) 
+         | SOME <> =>
+             #1 + "cnt_helper" "m" ("k"+#1)
+         end
+    ).
+
+  Definition cnt_map : expr:=
+    λ: "m" "n",
+      cnt_map_helper "m" #0 "n".
+      
+  Definition coupon_helper : expr :=
+    rec: "coupon_helper" "m" "n" "cnt" :=
+      if: cnt_map "m" "n" = "n" then !"cnt" else
+        "cnt" <- !"cnt" + #1;;
+        let: "k" := rand ("n" - #1) from #() in
+        set "m" "k" #();;
+        "coupon_helper" "m" "n" "cnt".
+        
+  Definition coupon_collection : expr :=
+    λ: "n",
+      let: "m" := init_map #() in
+      let: "cnt" := ref #0 in
+      coupon_helper "m" "n" "cnt". 
+
+  Definition spec_coupon_helper : expr :=
+    rec: "spec_coupon_helper" "t" "n" "cnt" :=
+      if: "n" = "t" then !"cnt" else
+        "cnt" <- !"cnt" + #1;;
+        let: "k" := rand ("n" - #1) from #() in
+        if: ("t" ≤ "k") then "spec_coupon_helper" ("t"+#1) "n" "cnt"
+        else "spec_coupon_helper" "t" "n" "cnt".
+  
+  Definition spec_coupon_collection : expr :=
+    λ: "n",
+      let: "t" := #0 in
+      let: "cnt" := ref #0 in
+      spec_coupon_helper "t" "n" "cnt".
+
 Section proofs.
   Context `{!clutchRGS Σ}.
 
   Definition couponN := nroot.@"coupon".
 
-  Definition check_map_helper : expr :=
-    (rec: "check_helper" "m" "k" "n" :=
-       if: "k" = "n"
-       then #true
-       else if: get "m" "k" = #1 then "check_helper" "m" ("k"+#1) else #false                
-    ).
+  (**  TODO! *)
+  Fixpoint cnt_gallina (vs: gmap nat val) (k:Z) (n:nat) := Z.of_nat 0.
 
-  Definition check_map : expr:=
-    λ: "m" "n",
-      check_map_helper "m" #0 "n".
-      
-  Definition coupon_helper : expr :=
-    rec: "coupon_helper" "m" "n" "cnt" :=
-      if: check_map "m" "n" then #() else
-        "cnt" <- !"cnt" + #1;;
-        let: "k" := rand "n" from #() in
-        set "m" "k" #1;;
-        "coupon_helper" "m" "n" "cnt".
-        
-  Definition coupon_collection : expr :=
-    λ: "n",
-      let: "m" := init_map in
-      set "m" "n" #();;
-      let: "cnt" := ref #0 in
-      coupon_helper "m" "n" "cnt";;
-      !"cnt".
+  (* This is an invariant in the sense that it holds true for every recursive call, 
+     but we do not technically allocate it as an invariant in the RA sense. 
+   *)
+  Definition coupon_collection_inv n m (k:Z) cnt cnt':= (∃(cntv : Z) lis , map_list m lis ∗ cnt' ↦ₛ #cntv ∗ cnt ↦ #cntv ∗ ⌜cnt_gallina lis 0 n = k⌝ )%I.
 
+  Lemma coupon_collection_refines_spec_helper n m (k:Z) cnt cnt':
+    ⊢ coupon_collection_inv n m k cnt cnt' -∗ REL coupon_helper #m #n #cnt << spec_coupon_helper #k #n #cnt' : lrel_nat.
+  Proof.
+    iLöb as "IH" forall (k).
+    iIntros "Inv".
+    iDestruct "Inv" as (??) "(?&?&?&%)".
+    rewrite {2}/coupon_helper {2}/spec_coupon_helper.
+    do 10 rel_pure_l. 
+    rewrite -!/cnt_map_helper.
+    rel_pures_r.
+    case_bool_decide.
+    - (* finish collecting*)
+      rel_pures_r. rel_load_r.
+      subst. 
+      inversion H0; subst. 
+      rel_apply_l (refines_wp_l _ _ (cnt_map_helper _ _ _)).
+    Admitted. 
+  
+  Lemma coupon_collection_refines_spec:
+    ⊢ REL coupon_collection << spec_coupon_collection : lrel_nat → lrel_nat.
+  Proof.
+    rel_arrow_val. iIntros (v1 v2 [n[-> ->]]) .
+    rel_pures_l.
+    rel_pures_r.
+    rel_alloc_r cnt' as "Hcnt'". do 2 rel_pure_r.
+    rel_apply_l (refines_wp_l _ _ (init_map #())).
+    wp_apply (wp_init_map with "[//]").
+    iIntros (m) "Hm".
+    rel_pures_l.
+    rel_alloc_l cnt as "Hcnt".
+    do 2 rel_pure_l.
+    rewrite -/coupon_helper -/spec_coupon_helper.
+    iApply (coupon_collection_refines_spec_helper with "[Hcnt' Hm Hcnt]").
+    rewrite /coupon_collection_inv; iExists _, _. iFrame.
+    by iPureIntro. 
+Qed. 
+
+  
+  
   
   
 End proofs.
